Fix to add callvalue to contract before executing And ensure no overflow or underflow in this transfer.

FunctionalCorrectness.v
@@ -186,9 +186,6 @@ Definition update_balances sender recipient amount balances : (addr -> Z) :=
      if Int256.eq a recipient then (balances recipient) + amount
       else (balances a).
 
-Definition extract_balances_from_me (ps_current : persistent_state) : addr -> Z := 
-  ps_balance ps_current.
-
 Definition update_ps_balance ps_before latest_balances : persistent_state :=
   mkPersistentState
   (ps_timestamp ps_before)
@@ -197,7 +194,7 @@ Definition update_ps_balance ps_before latest_balances : persistent_state :=
   (ps_blockhash ps_before)
 .
 
-Definition noOverflowInTransfer (sender recipient : addr) (amount : Z) (balances : addr -> Z) : bool := 
+Definition noOverflowOrUnderflowInTransfer (sender recipient : addr) (amount : Z) (balances : addr -> Z) : bool := 
   ((balances sender) - amount >=? 0)%Z
   && ((balances recipient) + amount <=? Int256.max_unsigned)%Z
 .
@@ -210,7 +207,7 @@ Definition ps_new_balance (ps_before : persistent_state) (d : global_abstract_da
     (ps_blockhash ps_before)
 .
 
-Definition extract_persistent_state (me : machine_env global_abstract_data_type) (d : global_abstract_data_type) : persistent_state :=
+Definition next_persistent_state (me : machine_env global_abstract_data_type) (d : global_abstract_data_type) : persistent_state :=
   mkPersistentState
     (me_timestamp me)
     (me_number me)
@@ -228,36 +225,52 @@ Definition execute_contract_call (* Note that this leaves blocknumber and timest
 match call with
 | NonExistentFunction => (d_before, ps_before)
 | CallFunction f origin caller callvalue coinbase chainid =>
-  let me_before := GenericMachineEnv.generic_machine_env
-  coinbase
-  (ps_timestamp ps_before)
-  (ps_number ps_before)
-  (ps_blockhash ps_before)
-  chainid
+  (* Ensure the transfer of callvalue to the contract doesn't overflow, if so revert. *)
+  if noOverflowOrUnderflowInTransfer caller contract_address callvalue (ps_balance ps_before)
+  then
+      let me := GenericMachineEnv.generic_machine_env
+      coinbase
+      (ps_timestamp ps_before)
+      (ps_number ps_before)
+      (ps_blockhash ps_before)
+      chainid
+      origin 
   origin 
-  contract_address
-  caller
-  callvalue
-  (ps_balance ps_before)
-  address_accepts_funds
+      origin 
+      contract_address
+      caller
+      callvalue
+      (update_balances caller contract_address callvalue (ps_balance ps_before))
+      address_accepts_funds
+      in
   in  
-  match f with
+      in
+      match f with
+      | contractStep_donate amount => 
     | contractStep_donate amount => 
-        match runStateT (Crowdfunding_donate_opt me_before) d_before with
-        | Some (_, d_after) => (d_after, extract_persistent_state me_before d_after)
-        | None => (d_before, ps_before)
-        end
+      | contractStep_donate amount => 
+          match runStateT (Crowdfunding_donate_opt me) d_before with
+          | Some (_, d_after) => 
+            (d_after, next_persistent_state me d_after)
+          | None => (d_before, ps_before) (* Revert *)
+          end
+      | contractStep_getFunds => 
     | contractStep_getFunds => 
-        match runStateT (Crowdfunding_getFunds_opt me_before) d_before with
-        | Some (_, d_after) => (d_after, extract_persistent_state me_before d_after)
-        | None => (d_before, ps_before)
-        end
+      | contractStep_getFunds => 
+          match runStateT (Crowdfunding_getFunds_opt me) d_before with
+          | Some (_, d_after) => (d_after, next_persistent_state me d_after)
+          | None => (d_before, ps_before) (* Revert *)
+          end
+      | contractStep_claim => 
     | contractStep_claim => 
-        match runStateT (Crowdfunding_claim_opt me_before) d_before with
-        | Some (_, d_after) => (d_after, extract_persistent_state me_before d_after)
-        | None => (d_before, ps_before)
-        end
-  end
+      | contractStep_claim => 
+          match runStateT (Crowdfunding_claim_opt me) d_before with
+          | Some (_, d_after) => (d_after, next_persistent_state me d_after)
+          | None => (d_before, ps_before) (* Revert *)
+          end
+    end
+  else
+    (d_before, ps_before) (* Revert due to overflow of contract_balance or insufficient funds in caller. *)
 end.
 
 Lemma OneTransferOnly : forall call d_before ps_before prf,
@@ -269,26 +282,30 @@ Lemma OneTransferOnly : forall call d_before ps_before prf,
     intros.
     destruct call eqn:Case.
     - simpl. rewrite H. auto.
-    - destruct f eqn:SCase;
-        (simpl;
-        match goal with
-        | [ |- context[runStateT ?X ]] => destruct (runStateT X) eqn:SSCase end;
-        [ destruct p;
-          (try (apply SingleTransferCheck.Crowdfunding_donate_opt_single_transfer with (d:=d_before) (coinbase:=coinbase) (timestamp:=ps_timestamp ps_before) (number:=ps_number ps_before) (blockhash:=ps_blockhash ps_before) (chainid:=chainid) (origin:=origin) (contract_address:=contract_address) (caller:=caller) (callvalue:=callvalue) (initial_balances:=ps_balance ps_before) (address_accepts_funds:=address_accepts_funds) (result:=u); [assumption | apply SSCase]);
-          try (apply SingleTransferCheck.Crowdfunding_getFunds_opt_single_transfer with (d:=d_before) (coinbase:=coinbase) (timestamp:=ps_timestamp ps_before) (number:=ps_number ps_before) (blockhash:=ps_blockhash ps_before) (chainid:=chainid) (origin:=origin) (contract_address:=contract_address) (caller:=caller) (callvalue:=callvalue) (initial_balances:=ps_balance ps_before) (address_accepts_funds:=address_accepts_funds) (result:=u); [assumption | apply SSCase]);
-          try (apply SingleTransferCheck.Crowdfunding_claim_opt_single_transfer with (d:=d_before) (coinbase:=coinbase) (timestamp:=ps_timestamp ps_before) (number:=ps_number ps_before) (blockhash:=ps_blockhash ps_before) (chainid:=chainid) (origin:=origin) (contract_address:=contract_address) (caller:=caller) (callvalue:=callvalue) (initial_balances:=ps_balance ps_before) (address_accepts_funds:=address_accepts_funds) (result:=u); [assumption | apply SSCase]))
-        |
-          rewrite H; auto
-        ])
-        .
-  Qed.
+    - unfold execute_contract_call.
+      destruct (noOverflowOrUnderflowInTransfer caller
+      contract_address callvalue
+      (ps_balance ps_before)).
+      + destruct f eqn:SCase;
+      (simpl;
+      match goal with
+      | [ |- context[runStateT ?X ]] => destruct (runStateT X) eqn:SSCase end;
+      [ destruct p;
+        (try (apply SingleTransferCheck.Crowdfunding_donate_opt_single_transfer with (d:=d_before) (coinbase:=coinbase) (timestamp:=ps_timestamp ps_before) (number:=ps_number ps_before) (blockhash:=ps_blockhash ps_before) (chainid:=chainid) (origin:=origin) (contract_address:=contract_address) (caller:=caller) (callvalue:=callvalue) (initial_balances:=(update_balances caller contract_address callvalue (ps_balance ps_before))) (address_accepts_funds:=address_accepts_funds) (result:=u); [assumption | apply SSCase]);
+        try (apply SingleTransferCheck.Crowdfunding_getFunds_opt_single_transfer with (d:=d_before) (coinbase:=coinbase) (timestamp:=ps_timestamp ps_before) (number:=ps_number ps_before) (blockhash:=ps_blockhash ps_before) (chainid:=chainid) (origin:=origin) (contract_address:=contract_address) (caller:=caller) (callvalue:=callvalue) (initial_balances:=(update_balances caller contract_address callvalue (ps_balance ps_before))) (address_accepts_funds:=address_accepts_funds) (result:=u); [assumption | apply SSCase]);
+        try (apply SingleTransferCheck.Crowdfunding_claim_opt_single_transfer with (d:=d_before) (coinbase:=coinbase) (timestamp:=ps_timestamp ps_before) (number:=ps_number ps_before) (blockhash:=ps_blockhash ps_before) (chainid:=chainid) (origin:=origin) (contract_address:=contract_address) (caller:=caller) (callvalue:=callvalue) (initial_balances:=(update_balances caller contract_address callvalue (ps_balance ps_before))) (address_accepts_funds:=address_accepts_funds) (result:=u); [assumption | apply SSCase]))
+      |
+        rewrite H; auto
+      ]).
+      + simpl. rewrite H. auto.
+Qed.
 
 Inductive BlockchainAction (ps_before : persistent_state) :=
   | contractExecution (c : ContractCall)
   | timePassing (block_count time_passing : int256)
                 (prf : validTimeChange block_count time_passing (ps_number ps_before) (ps_timestamp ps_before) = true)
   | externalBalanceTransfer (sender recipient : addr) (amount : Z)
-                            (prf : sender <> contract_address /\  noOverflowInTransfer sender recipient amount (extract_balances_from_me ps_before) = true)
+                            (prf : sender <> contract_address /\  noOverflowOrUnderflowInTransfer sender recipient amount (ps_balance ps_before) = true)
   | noOp.
 
 Record StepInfo := {
@@ -330,7 +347,7 @@ Program Definition step
   | timePassing block_count time_passing prf => 
       (d_before, updateTimeAndBlock ps_before block_count time_passing)
   | externalBalanceTransfer sender recipient amount prf =>
-      (d_before, update_ps_balance ps_before (updateBalances sender recipient amount (extract_balances_from_me ps_before)))
+      (d_before, update_ps_balance ps_before (update_balances sender recipient amount (ps_balance ps_before)))
   | noOp => (d_before, ps_before)
   end.
 
@@ -558,6 +575,14 @@ Proof.
       * destruct f eqn:SSCase.
         {
           unfold step in H0. simpl in H0.
+          destruct (noOverflowOrUnderflowInTransfer caller contract_address callvalue
+          (ps_balance ps_before));
+          [|
+            inversion H0;
+            unfold resetTransfers; unfold balance_backed; simpl;
+            unfold balance_backed in IHReachableState;
+            assumption
+          ].
           match goal with
           | H : context[runStateT ?X ] |- _ => destruct (runStateT X) eqn:SSSCase end; [|inversion H0; assumption].
           destruct p.
